riscV/CompilerAux.v
@@ -1,6 +1,6 @@
 Require Import String.
 Require Import Coqlib Errors.
-Require Import AST Linking Smallstep.
+Require Import AST Linking Smallstep Compiler0.
 Require Asm.
 (** RealAsm passed. *)
 (* Require RealAsmgen. *)
@@ -15,7 +15,7 @@ Require Asmlabelgen.
 Require Jumptablegen.
 (** Assembler passes *)
 Require Symbtablegen.
-Require Reloctablesgen.
+Require Reloctablesgen ReloctablesgenproofArchi.
 Require RelocBingen.
 (* Require AsmLongInt. *)
 (* Require MergeSection. *)
@@ -23,42 +23,14 @@ Require RelocBingen.
 Require RelocElfgen.
 Require EncodeRelocElf.
 
+Definition instr_size := Asm.instr_size_real.
+Definition instr_size_bound := Asm.instr_size_bound_real.
 
-(** * Composing the translation passes *)
-
-(** We first define useful monadic composition operators,
-    along with funny (but convenient) notations. *)
-
-Definition apply_total (A B: Type) (x: res A) (f: A -> B) : res B :=
-  match x with Error msg => Error msg | OK x1 => OK (f x1) end.
-
-Definition apply_partial (A B: Type)
-                         (x: res A) (f: A -> res B) : res B :=
-  match x with Error msg => Error msg | OK x1 => f x1 end.
-
-Notation "a @@@ b" :=
-   (apply_partial _ _ a b) (at level 50, left associativity).
-Notation "a @@ b" :=
-   (apply_total _ _ a b) (at level 50, left associativity).
-
-Definition print {A: Type} (printer: A -> unit) (prog: A) : A :=
-  let unused := printer prog in prog.
-
-Definition time {A B: Type} (name: string) (f: A -> B) : A -> B := f.
-
-Definition total_if {A: Type}
-          (flag: unit -> bool) (f: A -> A) (prog: A) : A :=
-  if flag tt then f prog else prog.
-
-Definition partial_if {A: Type}
-          (flag: unit -> bool) (f: A -> res A) (prog: A) : res A :=
-  if flag tt then f prog else OK prog.
+Lemma instr_eq_size: forall i1 i2,
+    ReloctablesgenproofArchi.instr_eq i1 i2 -> instr_size i1 = instr_size i2.
+Admitted.
 
 
-Section INSTR_SIZE.
-
-  Variable instr_size : Asm.instruction -> Z.
-  
   (** TargetPrinter *)
 Definition targetprinter p: res Asm.program :=
   OK p
@@ -81,16 +53,7 @@ Definition targetprinter p: res Asm.program :=
   (* @@ time "SSAsm" SSAsmproof.transf_program *)
   (* @@@ time "Translation from SSAsm to RealAsm" RealAsmgen.transf_program instr_size. *)
 
- 
- (** Assembler *)
- Definition assembler (p: Asm.program) :=
-  OK p
-  @@@ time "Generation of symbol table" Symbtablegen.transf_program instr_size
-  @@@ time "Generation of relocation table" Reloctablesgen.transf_program instr_size
-  @@@ time "Encoding of instructions and data" RelocBingen.transf_program
-  (* @@@ time "Merge Sections" MergeSection.transf_program *)
-  @@@ time "Generation of the reloctable Elf" RelocElfgen.gen_reloc_elf
-  @@@ time "Encoding of the reloctable Elf" EncodeRelocElf.encode_elf_file.
+
 
  (* without target printet, used to prove top theorem *)
  (* Definition transf_c_program_assembler1 (p: Csyntax.program) := *)
@@ -101,4 +64,61 @@ Definition targetprinter p: res Asm.program :=
  (*  (* @@@ time "Merge Sections" MergeSection.transf_program *) *)
  (*  @@@ time "Generation of the reloctable Elf" RelocElfgen.gen_reloc_elf *)
  (*  @@@ time "Encoding of the reloctable Elf" EncodeRelocElf.encode_elf_file. *)
-End INSTR_SIZE.
+
+Definition match_prog_targetprinter p tp :=
+  targetprinter p = OK tp.
+
+
+Lemma Pseudo_fn_stack_requirements_match: forall p,
+    fn_stack_requirements p = fn_stack_requirements (PseudoInstructions.transf_program p).
+Admitted.
+
+Lemma Fixup_fn_stack_requirements_match: forall p,
+    fn_stack_requirements p = fn_stack_requirements (AsmFixupcode.transf_program p).
+Admitted.
+
+Lemma BuiltInline_fn_stack_requirements_match: forall p tp,
+    AsmBuiltinInline.transf_program p = OK tp ->
+    fn_stack_requirements p = fn_stack_requirements tp.
+Admitted.
+
+Lemma AsmPseudo_fn_stack_requirements_match: forall p,
+    fn_stack_requirements p = fn_stack_requirements (AsmPseudoInstr.transf_program p).
+Admitted.
+
+Lemma Asmlabel_fn_stack_requirements_match: forall p tp,
+    Asmlabelgen.transf_program instr_size p = OK tp ->
+    fn_stack_requirements p = fn_stack_requirements tp.
+Admitted.  
+
+Lemma AsmLiteral_fn_stack_requirements_match: forall p,
+    fn_stack_requirements p = fn_stack_requirements (AsmLiteral.transf_program p).
+Admitted.
+
+    Lemma Jumptable_fn_stack_requirements_match: forall p,
+    fn_stack_requirements p = fn_stack_requirements (Jumptablegen.transf_program instr_size p).
+Admitted.
+
+
+Lemma targetprinter_fn_stack_requirements_match: forall p tp,
+    match_prog_targetprinter p tp ->
+    fn_stack_requirements p = fn_stack_requirements tp.
+Proof.
+  intros.
+  unfold match_prog_targetprinter in H. unfold targetprinter in H.
+  unfold time in H.
+  simpl in H. 
+  destruct  AsmBuiltinInline.transf_program eqn: T1; simpl in H; try discriminate.
+  destruct  Asmlabelgen.transf_program eqn: T2; simpl in H; try discriminate.
+  inv H.
+
+  rewrite Pseudo_fn_stack_requirements_match.
+  rewrite Fixup_fn_stack_requirements_match.
+  erewrite (BuiltInline_fn_stack_requirements_match _ _ T1).
+  rewrite AsmLiteral_fn_stack_requirements_match.
+  rewrite AsmPseudo_fn_stack_requirements_match.
+  erewrite (Asmlabel_fn_stack_requirements_match _ _ T2).
+  erewrite Jumptable_fn_stack_requirements_match.
+  auto.
+Qed.
+
