driver/Compiler0.v
@@ -1,0 +1,70 @@
+Require Import String.
+Require Import Coqlib Errors.
+Require Import AST Asm Globalenvs.
+Require Import RelocProg RelocProgram RelocElf RelocElfSemantics DecodeRelocElf.
+
+(** * Composing the translation passes *)
+
+(** We first define useful monadic composition operators,
+    along with funny (but convenient) notations. *)
+
+Definition apply_total (A B: Type) (x: res A) (f: A -> B) : res B :=
+  match x with Error msg => Error msg | OK x1 => OK (f x1) end.
+
+Definition apply_partial (A B: Type)
+                         (x: res A) (f: A -> res B) : res B :=
+  match x with Error msg => Error msg | OK x1 => f x1 end.
+
+Notation "a @@@ b" :=
+   (apply_partial _ _ a b) (at level 50, left associativity).
+Notation "a @@ b" :=
+   (apply_total _ _ a b) (at level 50, left associativity).
+
+Definition print {A: Type} (printer: A -> unit) (prog: A) : A :=
+  let unused := printer prog in prog.
+
+Definition time {A B: Type} (name: string) (f: A -> B) : A -> B := f.
+
+Definition total_if {A: Type}
+          (flag: unit -> bool) (f: A -> A) (prog: A) : A :=
+  if flag tt then f prog else prog.
+
+Definition partial_if {A: Type}
+          (flag: unit -> bool) (f: A -> res A) (prog: A) : res A :=
+  if flag tt then f prog else OK prog.
+
+
+(* stack requirements *)
+
+Definition fn_stack_requirements (tp: Asm.program) (id: ident) : Z :=
+    match Globalenvs.Genv.find_funct_ptr (Globalenvs.Genv.globalenv tp) (Values.Global id) with
+    | Some (Internal f) => Asm.fn_stacksize f
+    | _ => 0
+    end.
+
+(* CCELF Start *)
+Definition reloc_fn_stack_requirements {I D: Type} (tp: RelocProg.program Asm.fundef unit I D) (id:ident) : Z :=
+  match List.find (fun '(id',_) => ident_eq id id') (RelocProg.prog_defs tp) with
+  | None => 0
+  | Some (_, def) =>
+    match def with
+    | (Gfun (Internal f)) => Asm.fn_stacksize f
+    | _ => 0
+    end
+  end.
+
+Definition elf_fn_stack_requirements (tp: RelocElf.elf_file) (id:ident) : Z :=
+  match (RelocElfSemantics.decode_elf tp) with
+  | OK p =>
+    reloc_fn_stack_requirements p id
+  | _ => 0
+  end.
+  
+Definition elf_bytes_stack_requirements (tp: list Integers.Byte.int * Asm.program * Globalenvs.Senv.t)
+           (id:ident) : Z :=
+  let '(b, p, s) := tp in
+  match DecodeRelocElf.decode_elf_file b p s with
+  | OK ef => elf_fn_stack_requirements ef id
+  | _ => 0
+  end.
+(* CCELF End *)
